proof/agp32CorrectScript.sml
@@ -1,4 +1,4 @@
-open hardwarePreamble translatorTheory translatorLib arithmeticTheory dep_rewrite blastLib bitstringSyntax fcpSyntax listSyntax wordsSyntax agp32StateTheory agp32EnvironmentTheory agp32ProcessorTheory ag32Theory ag32ExtraTheory agp32RelationTheory;
+open hardwarePreamble translatorTheory translatorLib arithmeticTheory dep_rewrite blastLib bitstringSyntax fcpSyntax listSyntax wordsSyntax agp32StateTheory agp32EnvironmentTheory agp32ProcessorTheory ag32Theory ag32ExtraTheory ag32UtilitiesTheory agp32RelationTheory agp32UpdateTheory;
 
 val _ = new_theory "agp32Correct";
 
@@ -10,97 +10,23 @@ val _ = new_theory "agp32Correct";
 val _ = prefer_num ();
 val _ = guess_lengths ();
 
-fun v2w_word_bit_list_cleanup tm =
-  if is_var tm orelse is_const tm then
-    raise UNCHANGED
-  else if is_v2w tm andalso (is_list (rand tm)) then let
-    val (arg, worddim) = dest_v2w tm
-    val (arg, _) = dest_list arg
-    val len = length arg
-  in
-    if len = 1 then
-      raise UNCHANGED
-    else let
-      (* TODO: Fails on lists of non-dest_word_bit calls *)
-      val (hindex, var) = arg |> hd |> dest_word_bit
-      val (lindex, _) = arg |> last |> dest_word_bit
-    in
-      mk_eq (tm, mk_word_extract (hindex, lindex, var, mk_int_numeric_type len)) |> BBLAST_PROVE
-    end
-  end else if is_comb tm then
-    COMB_CONV v2w_word_bit_list_cleanup tm
-  else (* must be abs *)
-    ABS_CONV v2w_word_bit_list_cleanup tm;
-
-(* lemmas about the Silver ISA *)
-Theorem ALU_state_eq_after:
-  !func input1 input2 res a a'.
-    ALU (func, input1, input2) a = (res, a') ==>
-    a'.PC = a.PC /\ a'.MEM = a.MEM /\ a'.PC = a.PC /\ a'.R = a.R /\
-    a'.data_in = a.data_in /\ a'.data_out = a.data_out /\ a'.io_events = a.io_events
-Proof
-  rw [ALU_def] >> Cases_on `func'` >> fs [] >> rw []
-QED
-
-Theorem ag32_data_in_unchanged:
-  !a n. (FUNPOW Next n a).data_in = (FUNPOW Next (SUC n) a).data_in
-Proof
-  rw [FUNPOW_SUC] >>
-  Q.ABBREV_TAC `a1 = FUNPOW Next n a` >>
-  rw [Next_def] >>
-  Q.ABBREV_TAC `i = (a1.MEM ((31 >< 2) a1.PC @@ (0w:word2) + 3w) @@
-                     a1.MEM ((31 >< 2) a1.PC @@ (0w:word2) + 2w) @@
-                     a1.MEM ((31 >< 2) a1.PC @@ (0w:word2) + 1w) @@
-                     a1.MEM ((31 >< 2) a1.PC @@ (0w:word2)))` >>
-  rw [Decode_def,boolify32_def] >> CONV_TAC v2w_word_bit_list_cleanup >>
-  rw [Run_def,dfn'LoadUpperConstant_def,dfn'LoadConstant_def,
-      dfn'Interrupt_def,incPC_def] >-
-   (** JumpIfZero **)
-   (rw [dfn'JumpIfZero_def] >>
-    qpat_abbrev_tac `alu = ALU _ _` >>
-    Cases_on `alu` >> rw [incPC_def] >>
-    METIS_TAC [ALU_state_eq_after]) >-
-   (** JumpIfNotZero **)
-    (rw [dfn'JumpIfNotZero_def] >>
-     qpat_abbrev_tac `alu = ALU _ _` >>
-     Cases_on `alu` >> rw [incPC_def] >>
-     METIS_TAC [ALU_state_eq_after]) >>
-  Cases_on `DecodeReg_imm (v2w [word_bit 31 i],(30 >< 25) i)` >> rw [] >>
-  (** Other instructions **)
-  rw [dfn'Normal_def,norm_def,dfn'Shift_def,incPC_def,dfn'StoreMEM_def,
-      dfn'StoreMEMByte_def,dfn'LoadMEM_def,dfn'LoadMEMByte_def,
-      dfn'Out_def,dfn'In_def,dfn'Accelerator_def,dfn'Jump_def] >>
-  qpat_abbrev_tac `alu = ALU _ _` >>
-  Cases_on `alu` >> rw [] >>
-  METIS_TAC [ALU_state_eq_after]
-QED
-
+(* Init relation implies Rel at cycle 0 *)
 Theorem agp32_Init_implies_Rel:
   !k fext fbits s a I.
     k >= 1 ==>
     k <= 5 ==>
     s = agp32 fext fbits ==>
-    is_mem fext_accessor_circuit s fext ==>
-    is_acc accelerator_f s ==>
-    is_interrupt_interface fext_accessor_circuit s fext ==>
-    Init (fext 0) (s 0) a ==>
     I(k,0) = 0 ==>
-    Rel (fext 0) (s 0) k a 0
+    Init (fext 0) (s 0) a ==>
+    Rel (fext 0) (s 0) I 0 a 0
 Proof
   rpt strip_tac >>
-  fs [Init_def,Rel_def] >>
-  Cases_on `k = 1` >-
-   (fs [] >> cheat) >>
-  Cases_on `k = 2` >-
-   (fs [] >> cheat) >>
-  Cases_on `k = 3` >-
-   (fs [] >> cheat) >>
-  Cases_on `k = 4` >-
-   (fs [] >> cheat) >>
-  Cases_on `k = 5` >-
-   (fs [] >> cheat) >> fs []
+  fs [Init_def,Rel_def] >> rw [] >-
+   cheat >>
+  fs [enable_stg_def] >> fs []
 QED
 
+(* correctness of the pipelined Silver concerning the ISA *)
 Theorem agp32_Rel_ag32_correct:
   !k fext fbits s a (t:num) I C.
     k >= 1 ==>
@@ -117,21 +43,29 @@ Theorem agp32_Rel_ag32_correct:
     (** properties of scheduling function I **)
     (!t k. enable_stg k (s (SUC t)) ==> I(k,SUC t) = I(k,t) + 1) ==>
     I(k,0) = 0 ==>
-    Rel (fext t) (s t) k a (I(k,t))
+    Rel (fext t) (s t) I t a (I(k,t))
 Proof
-  rpt strip_tac >>
-  Induct_on `t` >> fs [] >-
+  Induct_on `t` >>
+  rpt strip_tac >-
    METIS_TAC [agp32_Init_implies_Rel] >>
-  Q.ABBREV_TAC `i = I'(k,t)` >>
+  `Rel (fext t) (s t) I' t a (I' (k,t))` by METIS_TAC [] >>
+  Q.ABBREV_TAC `i = I'(k,t)` >> 
   Cases_on `enable_stg k (s (SUC t))` >-
    (`I'(k, SUC t) = SUC i` by fs [] >> fs [Rel_def] >>
     Cases_on `k = 1` >-
      (** IF stage **)
-     (fs [] >> rw [] >|[
-         fs [GSYM ag32_data_in_unchanged,is_data_in_def],
-         rw [agp32_def,mk_module_def] >> cheat,
-         cheat]) >>
-      cheat) >>
+     (fs [] >> rw [] >-
+       fs [GSYM ag32_data_in_unchanged,is_data_in_def] >>
+      `I'(1,SUC t) <> I'(2,SUC t)` by cheat >> fs [] >>
+      `I'(1,SUC t) <> I'(3,SUC t)` by cheat >> fs [] >>
+      `I'(1,SUC t) <> I'(4,SUC t)` by cheat >> fs [] >>
+      `I'(1,SUC t) <> I'(5,SUC t)` by cheat >> fs [] >>
+      rw [IF_Rel_def] >>
+      `?s s'. (agp32 fext fbits (SUC t)).IF.IF_instr =
+      (IF_instr_update (fext (SUC t)) s s').IF.IF_instr`
+        by rw [agp32_IF_instr_updated_by_IF_instr_update] >>
+      rw [IF_instr_update_def,instr_def] >> cheat) >>
+    cheat) >>
   cheat
 QED
 
